ulib/FStar.Pervasives.fst
@@ -78,6 +78,8 @@ let commute_nested_matches = ()
 
 let noextract_to _ = ()
 
+let ite_soundness_by = ()
+
 let normalize_term #_ x = x
 
 let normalize a = a
